\item Prove that 
\begin{align*}
    &\phantom{{}={}} P(E \cup F \cup G)\\
    &= P(E) + P(F) + P(G) - {}\\
    &\phantom{{}={}} P(E^cFG) - P(EF^cG) - P(EFG^c) - {}\\
    &\phantom{{}={}} 2 P(EFG)
\end{align*}

\begin{proof}[Demostraci√≥n] de la equivalencia anterior.
    \begin{align*}
        &\phantom{{}={}} P(E \cup F \cup G)\\
        &= P(E) + P(F \cup G) - P(E (F \cup G))\\
        &= P(E) + P(F) + P(G) - {}\\
        &\phantom{{}={}} P(FG) - P(E (F \cup G))\\
        &= P(E) + P(F) + P(G) - {}\\
        &\phantom{{}={}} P(FG) - P((E F) \cup (E G))\\
        &= P(E) + P(F) + P(G) - {}\\
        &\phantom{{}={}} P(FG) - P(EF) - P(EG) + P(EFG)\\
        &= P(E) + P(F) + P(G) - {}\\
        &\phantom{{}={}} (P(EFG) P(E^cFG)) - {}\\
        &\phantom{{}={}} (P(EFG) + P(EFG^c)) - {}\\
        &\phantom{{}={}} (P(EFG) + P(EF^cG)) + {}\\
        &\phantom{{}={}} P(EFG)\\
        &= P(E) + P(F) + P(G) - 3 P(EFG) - {}\\
        &\phantom{{}={}} P(E^cFG) - P(EFG^c) - P(EF^cG) + {}\\
        &\phantom{{}={}} P(EFG)\\
        &= P(E) + P(F) + P(G) - {}\\
        &\phantom{{}={}} P(E^cFG) - P(EFG^c) - P(EF^cG) - {}\\
        &\phantom{{}={}} 2 P(EFG) \qedhere
    \end{align*}
    
\end{proof}