\item $F = FE \cup FE^\complement $ and $E \cup F = E \cup E^\complement F$.

\begin{proof}[Demostración] de la relación anterior.

    \begin{align*}
        F &= FS\\
        &= F (E\cup E^\complement )\\
        &= FE \cup F E^\complement 
        \shortintertext{y}
        E \cup F &= (E \cup F)(E\cup E^\complement )\\
        &= ((E\cup F)E) \cup ((E\cup F)E^\complement )\\
        &= E \cup ((E^\complement  E)\cup(E^\complement  F))\\
        &= E \cup (\varnothing\cup(E^\complement  F))\\
        &= E \cup E^\complement  F \qedhere
    \end{align*}
\end{proof}